flag for relocbindecode

driver/Compiler.v
@@ -216,7 +216,7 @@ Definition transf_c_program_real p : res Asm.program :=
   @@@ time "Translation from RawAsm to RealAsm" RealAsmgen.transf_program
   @@@ PseudoInstructions.check_program
   @@ time "Elimination of pseudo instruction" PseudoInstructions.transf_program.
-Definition transf_c_program_bytes (p: Csyntax.program) : res (list Integers.byte * Asm.program * Globalenvs.Senv.t) :=
+Definition transf_c_program_bytes (more: bool)(p: Csyntax.program) : res (list Integers.byte * Asm.program * Globalenvs.Senv.t) :=
   transf_c_program_real p
   @@@ time "Make local jumps use offsets instead of labels" Asmlabelgen.transf_program
   @@ time "Pad Nops to make the alignment of functions correct" PadNops.transf_program
@@ -224,7 +224,7 @@ Definition transf_c_program_bytes (p: Csyntax.program) : res (list Integers.byte
   @@@ time "Generation of the symbol table" Symbtablegen.transf_program
   (* @@@ time "Normalize the symbol table indexes" NormalizeSymb.transf_program *)
   @@@ time "Generation of relocation table" Reloctablesgen.transf_program
-  @@@ time "Encoding of instructions and data" (RelocBingen.transf_program true)
+  @@@ time "Encoding of instructions and data" (RelocBingen.transf_program more)
   (* @@@ time "Added the starting stub code" Stubgen.transf_program *)
   @@ time "Removing addendums" RemoveAddend.transf_program
   @@@ time "Encoding of tables" TablesEncode.transf_program
@@ -247,14 +247,14 @@ Definition transf_c_program_bytes_more (p: Csyntax.program) : res (list Integers
   @@@ time "Generation of the reloctable Elf" RelocElfgen.gen_reloc_elf
   @@@ time "Encoding of the reloctable Elf" EncodeRelocElf.encode_elf_file.  
 
-Definition transf_c_program_bytes' (p: Csyntax.program) :=
+Definition transf_c_program_bytes' (more: bool) (p: Csyntax.program) :=
   transf_c_program_real p
   @@@ time "Make local jumps use offsets instead of labels" Asmlabelgen.transf_program
   @@ time "Pad Nops to make the alignment of functions correct" PadNops.transf_program
   @@ time "Pad space to make the alignment of data correct" PadInitData.transf_program
   @@@ time "Generation of the symbol table" Symbtablegen.transf_program
   @@@ time "Generation of relocation table" Reloctablesgen.transf_program
-  @@@ time "Encoding of instructions and data" (RelocBingen.transf_program true)
+  @@@ time "Encoding of instructions and data" (RelocBingen.transf_program more)
   @@ time "Removing addendums" RemoveAddend.transf_program
   @@@ time "Encoding of tables" TablesEncode.transf_program
   @@@ time "Generation of the reloctable Elf" RelocElfgen.gen_reloc_elf
@@ -552,7 +552,7 @@ Qed.
 
 Theorem transf_c_program_bytes_match :
   forall p tp,
-    transf_c_program_bytes' p = OK tp ->
+    transf_c_program_bytes' false p = OK tp ->
     match_prog_bytes p tp.
 Proof.
   intros p tp T. unfold transf_c_program_bytes' in T.
@@ -561,7 +561,7 @@ Proof.
   destruct (Asmlabelgen.transf_program p1) eqn:RTP; simpl in T; try discriminate.
   destruct (Symbtablegen.transf_program (PadInitData.transf_program (PadNops.transf_program p0))) eqn:STG; simpl in T; try discriminate.
   destruct (Reloctablesgen.transf_program p2) eqn: RTG; simpl in T; try discriminate.
-  destruct (RelocBingen.transf_program true p3) eqn: RBG; simpl in T; try discriminate.
+  destruct (RelocBingen.transf_program false p3) eqn: RBG; simpl in T; try discriminate.
   destruct (TablesEncode.transf_program (RemoveAddend.transf_program p4)) eqn: TE; simpl in T; try discriminate.
   destruct (RelocElfgen.gen_reloc_elf p5) eqn:GRE; simpl in T; try discriminate.
   red.
@@ -1237,7 +1237,7 @@ Qed.
 
 Theorem transf_c_program_correct_bytes:
   forall p b tp s,
-    transf_c_program_bytes' p = OK (b, tp, s) ->
+    transf_c_program_bytes' false p = OK (b, tp, s) ->
     backward_simulation (Csem.semantics (elf_bytes_stack_requirements (b,tp,s)) p) (ElfBytesSemantics.semantics b tp s (Asm.Pregmap.init Values.Vundef)).
 Proof.
   intros. exploit c_semantic_preservation_bytes. apply transf_c_program_bytes_match; eauto.
